fstar/MLS.TreeDEM.Message.Transcript.fst
@@ -7,37 +7,29 @@ open MLS.TreeDEM.Message.Content
 open MLS.Result
 open MLS.Crypto
 
-val compute_confirmed_transcript_hash: #bytes:Type0 -> {|crypto_bytes bytes|} -> message bytes -> bytes -> bytes -> result (lbytes bytes (hash_length #bytes))
+val compute_confirmed_transcript_hash: #bytes:Type0 -> {|crypto_bytes bytes|} -> message_content bytes -> bytes -> bytes -> result (lbytes bytes (hash_length #bytes))
 let compute_confirmed_transcript_hash #bytes #cb msg signature interim_transcript_hash =
-  if not (length msg.group_id < 256) then
-    internal_failure "compute_confirmed_transcript_hash: group_id too long"
-  else if not (msg.epoch < pow2 64) then
-    internal_failure "compute_confirmed_transcript_hash: epoch too big"
-  else if not (length msg.authenticated_data < pow2 32) then
-    internal_failure "compute_confirmed_transcript_hash: authenticated_data too long"
-  else if not (length signature < pow2 16) then
+  if not (length signature < pow2 16) then
     internal_failure "compute_confirmed_transcript_hash: signature too long"
-  else if not (msg.content_type = CT_commit) then
+  else if not (msg.content_type = CT_commit ()) then
     internal_failure "compute_confirmed_transcript_hash: should only be used on a commit message"
   else (
-    sender <-- sender_to_network msg.sender;
-    content <-- message_content_pair_to_network msg.message_content;
-    let serialized_msg = serialize (mls_plaintext_commit_content_nt bytes) ({
-      wire_format = wire_format_to_network msg.wire_format;
-      group_id = msg.group_id;
-      epoch = msg.epoch;
-      sender = sender;
-      authenticated_data = msg.authenticated_data;
-      content = content;
+    msg_network <-- message_content_to_network #bytes #cb msg;
+    let serialized_msg = serialize (mls_message_commit_content_nt bytes) ({
+      wire_format = msg.wire_format;
+      content = msg_network;
       signature = signature;
     }) in
     hash_hash (concat interim_transcript_hash serialized_msg)
   )
 
-val compute_interim_transcript_hash: #bytes:Type0 -> {|crypto_bytes bytes|} -> option bytes -> bytes -> result (lbytes bytes (hash_length #bytes))
+val compute_interim_transcript_hash: #bytes:Type0 -> {|crypto_bytes bytes|} -> bytes -> bytes -> result (lbytes bytes (hash_length #bytes))
 let compute_interim_transcript_hash #bytes #cb confirmation_tag confirmed_transcript_hash =
-  confirmation_tag_network <-- opt_bytes_to_opt_tag confirmation_tag;
-  let serialized_auth = serialize (mls_plaintext_commit_auth_data_nt bytes) ({
-    confirmation_tag = confirmation_tag_network;
-  }) in
-  hash_hash (concat confirmed_transcript_hash serialized_auth)
+  if not (length confirmation_tag < 256) then
+    internal_failure "compute_interim_transcript_hash: confirmation_tag too long"
+  else (
+    let serialized_auth = serialize (mls_message_commit_auth_data_nt bytes) ({
+      confirmation_tag = {mac_value = confirmation_tag};
+    }) in
+    hash_hash (concat confirmed_transcript_hash serialized_auth)
+  )
